Simu/Cor.v
@@ -18,23 +18,6 @@ Section SIMU.
   (* Hypothesis WF: well_formed prog. *)
   Hypothesis MAINNODE: find_class main_node prog = Some (c_main, cls_main).
 
-
-  (* Inductive match_states: state * stmt * cont -> Clight.state -> Prop := *)
-  (* | intro_state: forall me ve s k k' e le m, *)
-  (*     compat_venv c_main ve e m -> *)
-  (*     compat_menv main_node tprog c_main me e m -> *)
-  (*     well_formed_stmt c_main s -> *)
-  (*     compat_stmt main_node tprog me ve e m s -> *)
-  (*     compat_cont k k' -> *)
-  (*     mem_sep main_node c_main e m -> *)
-  (*     self_sep main_node e m -> *)
-  (*     fields_sep tprog m -> *)
-  (*     nodup_env e -> *)
-  (*     nodup_vars c_main -> *)
-  (*     nodup_mems c_main -> *)
-  (*     match_states *)
-  (*       ((me, ve), s, k) *)
-  (*       (Clight.State (main_fun main_node c_main) (translate_stmt main_node s) k' e le m). *)
      
   Inductive match_states: state -> Clight.state -> Prop :=
     intro_state: forall me ve s k e le m,
@@ -58,6 +41,14 @@ Section SIMU.
            state_context (me, ve, Assign x e) k env le m
        | ctxt_stassign: forall me ve x e k env le m,
            state_context (me, ve, AssignSt x e) k env le m
+       | ctxt_ifte: forall me ve e v b s1 s2 k env le m,
+           exp_eval me ve e v ->
+           Cop.bool_val v (typeof e) m = Some b ->
+           match_states
+             (me, ve, if b then s1 else s2)
+             (Clight.State (main_fun main_node c_main)
+                           (translate_stmt main_node (if b then s1 else s2)) k env le m) ->
+           state_context (me, ve, Ifte e s1 s2) k env le m
        | ctxt_comp: forall me1 ve1 s1 me2 ve2 s2 me3 ve3 k e le m m' m'',
            match_states
              (me1, ve1, s1)
@@ -93,11 +84,14 @@ Section SIMU.
   Hint Resolve expr_eval_simu Clight.assign_loc_value sem_cast_same.
   Hint Constructors compat_stmt state_context.
 
-  Ltac discriminate' :=
-    match goal with
-    | H: ?x <> ?x |- _ => contradict H; reflexivity
-    end.
-  
+  Remark ifte_translate:
+    forall (b: bool) s1 s2,
+      translate_stmt main_node (if b then s1 else s2) =
+      if b then (translate_stmt main_node s1) else (translate_stmt main_node s2).
+  Proof.
+    now destruct b.
+  Qed.
+    
   Theorem simu:
     forall S1 S2,
       stmt_eval S1 S2 ->
@@ -115,16 +109,16 @@ Section SIMU.
     (* Assign x e : "x = e" *)
     - app_exp_eval_det.
       edestruct compat_assign_pres as [m']; eauto; destruct_conjs. 
-      exists (Clight.State (main_fun main_node c_main) Clight.Sskip k e0 le m'), Events.E0; split.
+      do 2 econstructor; split.
       + eapply Smallstep.plus_one, Clight.step_assign; eauto.
         * eapply expr_eval_simu; eauto.
         * rewrite type_pres; auto. 
-      + constructor; (tauto || auto). 
+      + constructor; auto. 
         
     (* AssignSt x e : "self->x = e"*)
     - app_exp_eval_det.
-      edestruct compat_stassign_pres as [m']; eauto; destruct_conjs. 
-      exists (Clight.State (main_fun main_node c_main) Clight.Sskip k e0 le m'), Events.E0; split.
+      edestruct compat_stassign_pres as [m']; eauto; destruct_conjs.
+      do 2 econstructor; split.
       + eapply Smallstep.plus_one, Clight.step_assign; eauto.
         *{ eapply Clight.eval_Efield_struct
            with (id:=main_node) (att:=Ctypes.noattr); eauto.
@@ -136,17 +130,25 @@ Section SIMU.
          }
         * eapply expr_eval_simu; eauto.
         * rewrite type_pres; auto. 
-      + constructor; (tauto || auto). 
+      + constructor; auto.
 
+    (* Ifte e s1 s2 : "if e then s1 else s2" *)
+    - app_exp_eval_det.
+      pose proof (bool_val_ptr v _ m0 m H0) as Hptr.
+      rewrite Hptr in H24. rewrite H1 in H24; inversion H24; subst b0; clear H24.
+      edestruct IHstmt_eval as [S2' [t1 [Step1 ?]]]; eauto.
+      do 2 econstructor; split; eauto.
+      eapply Smallstep.plus_left'; eauto.
+      rewrite ifte_translate.
+      eapply Clight.step_ifthenelse.
+      + eapply expr_eval_simu; eauto.
+      + erewrite type_pres, bool_val_ptr; eauto.  
+      
     (* Comp s1 s2 : "s1; s2" *)
     - repeat app_stmt_eval_det.
       edestruct IHstmt_eval1 as [S2' [t1 [Step1 ?]]]; eauto.
       edestruct IHstmt_eval2 as [S3' [t2 [Step2 ?]]]; eauto.
-      assert (S2' = Clight.State (main_fun main_node c_main)
-               (translate_stmt main_node Skip)
-               (Clight.Kseq (translate_stmt main_node s2) k) e le m'). admit. subst S2'.
-      assert (S3' = Clight.State (main_fun main_node c_main) (translate_stmt main_node Skip) k e le m''). admit. subst S3'.
-      exists (Clight.State (main_fun main_node c_main) (translate_stmt main_node Skip) k e le m''), Events.E0; split; auto.
+      do 2 econstructor; split; eauto.
       eapply Smallstep.plus_left' with
       (s2:=Clight.State (main_fun main_node c_main) (translate_stmt main_node s1)
                         (Clight.Kseq (translate_stmt main_node s2) k) e le m)
@@ -156,7 +158,10 @@ Section SIMU.
         *{ eapply Smallstep.plus_left' with
           (s2:=Clight.State (main_fun main_node c_main) (translate_stmt main_node s2) k e le m')
             (t1:=Events.E0) (t2:=Events.E0); auto.
-           - apply Clight.step_skip_seq.
+           - assert (S2' = Clight.State (main_fun main_node c_main)
+                                        (translate_stmt main_node Skip)
+                                        (Clight.Kseq (translate_stmt main_node s2) k) e le m'). admit. subst S2'.
+             apply Clight.step_skip_seq.
            - assert (t2 = Events.E0). admit. subst t2; auto.
          }
         * assert (t1 = Events.E0). admit. subst t1; auto.
@@ -164,16 +169,13 @@ Section SIMU.
     (* Comp Skip s : "skip; s" *)
     - repeat app_stmt_eval_det.
       edestruct IHstmt_eval as [S2' [t1 [Step1 Match2]]]; eauto.
-      assert (S2' = Clight.State (main_fun main_node c_main) (translate_stmt main_node Skip) k e le m'). admit. subst S2'.
-      exists (Clight.State (main_fun main_node c_main) (translate_stmt main_node Skip) k e le m'), Events.E0; split; auto.
+      do 2 econstructor; split; eauto.
       eapply Smallstep.plus_left' with
       (s2:=Clight.State (main_fun main_node c_main) (translate_stmt main_node Skip)
                         (Clight.Kseq (translate_stmt main_node s) k) e le m)
-        (t1:=Events.E0) (t2:=Events.E0); auto.
+        (t1:=Events.E0) (t2:=Events.E0); eauto.
       + eapply Clight.step_seq.
-      + eapply Smallstep.plus_left' with
-        (s2:=Clight.State (main_fun main_node c_main) (translate_stmt main_node s) k e le m)
-          (t1:=Events.E0) (t2:=Events.E0); auto.
+      + eapply Smallstep.plus_left'; eauto.
         * apply Clight.step_skip_seq.
         * assert (t1 = Events.E0). admit. subst t1; auto.
   Qed.
